Proved an invariant about get_var with injective f

new-backend/word_procScript.sml
@@ -2,11 +2,6 @@ open HolKernel Parse boolLib bossLib;
 
 val _ = new_theory "word_proc";
 
-open pred_setTheory arithmeticTheory pairTheory listTheory combinTheory;
-open finite_mapTheory sumTheory relationTheory stringTheory optionTheory;
-open wordsTheory sptreeTheory lcsymtacs bvpTheory;
-open word_langTheory
-
 (*Coloring expressions*)
 val apply_color_exp_def = tDefine "apply_color_exp" `
   (apply_color_exp f (Var num) = Var (f num)) /\
@@ -19,9 +14,11 @@ val apply_color_exp_def = tDefine "apply_color_exp" `
   \\ TRY (FIRST_X_ASSUM (ASSUME_TAC o Q.SPEC `ARB`))
   \\ DECIDE_TAC);
 
-(*Apply f to the keys of a num_map*)
-val apply_key_numset_def = Define `
-  (apply_numset f nummap = fromAList (MAP (\x,y.f x,y) (toAList nummap)))`
+(*Apply f to the keys of a num_map, numsets are special cases with val = ()*)
+val apply_nummap_key_def = Define `
+  apply_nummap_key f nummap = fromAList (
+                                 ZIP (MAP (f o FST) (toAList nummap),
+                                      MAP SND (toAList nummap)))`
 
 (*TODO: Coloring a prog*)
 val apply_color_def = Define `
@@ -33,7 +30,7 @@ val apply_color_def = Define `
   (apply_color f (Call ret dest args h) = 
     let ret = case ret of NONE => NONE 
                         | SOME (v,cutset) => 
-                             SOME (f v,apply_numset f cutset) in
+                             SOME (f v,apply_nummap_key f cutset) in
     let dest = case dest of NONE => NONE
                           | SOME n => SOME (f n) in
     let args = MAP f args in
@@ -43,13 +40,16 @@ val apply_color_def = Define `
   (apply_color f (Seq s1 s2) = Seq (apply_color f s1) (apply_color f s2)) /\
   (apply_color f (If e1 num e2 e3) = 
     If (apply_color f e1) (f num) (apply_color f e2) (apply_color f e3)) /\
-  (*Need a map over numsets*)
-  (apply_color f (Alloc num numset) = Alloc (f num) (apply_numset f numset)) /\
+  (apply_color f (Alloc num numset) = 
+    Alloc (f num) (apply_nummap_key f numset)) /\
   (apply_color f (Raise num) = Raise (f num)) /\
   (apply_color f (Return num) = Return (f num)) /\ 
-  (apply_color f Tick = Tick)/\
+  (apply_color f Tick = Tick) /\
+  (apply_color f (Set n exp) = Set n (apply_color_exp f exp)) /\
   (apply_color f p = p )
 `
+val _ = export_rewrites ["apply_nummap_key_def","apply_color_exp_def","apply_color_def"];
+
 (*
 EVAL ``apply_color (\x.x+1) (Seq (Call (SOME (5,LN)) (SOME 4) [3;2;1] NONE) Skip)``
 *)
@@ -125,16 +125,15 @@ val move_conv_lemma = store_thm ("move_conv_lemma",
     first_x_assum(qspec_then`h`mp_tac) >>
     simp[]>> fs[domain_lookup]>>
     strip_tac>> fs[] )
-
   >>
-    Cases_on `get_vars l s` >> fs[])>>
   Q.UNABBREV_TAC `args`>>
   rw[wEval_def]>-
     (fs[listTheory.MAP_ZIP,listTheory.ALL_DISTINCT_SET_TO_LIST,
        listTheory.ALL_DISTINCT_MAP_INJ,INJ_DEF,listTheory.MEM_SET_TO_LIST]>> 
     first_x_assum(qspec_then`SET_TO_LIST (domain s.locals)`mp_tac) >>
     simp[] >> Q.ABBREV_TAC `args = SET_TO_LIST (domain s.locals)`>>
-    rw[] >>
+    rw[set_vars_def,list_insert_def] >> simp[]
+    
     Cases_on `get_vars args s` >>
     fs[] ) >>
   fs[MAP_ZIP,ALL_DISTINCT_MAP_INJ,ALL_DISTINCT_SET_TO_LIST]>>
@@ -142,6 +141,287 @@ val move_conv_lemma = store_thm ("move_conv_lemma",
   match_mp_tac ALL_DISTINCT_MAP_INJ>> simp[]>>
   fs[INJ_DEF] );
 
+(*Prove a side result about fromAList: 
+  The keys in the Alist will always be in the resulting domain*)
+
+val MEM_fromAList = store_thm ("MEM_fromAList",
+  ``∀t k. MEM k (MAP FST t) <=> 
+          k IN domain (fromAList (t :(num,'a word_loc) env))``,
+  Induct_on`t`>>
+    rw[fromAList_def]>>
+  Cases_on`h`>> 
+  Cases_on`q=k`>>
+    rw[fromAList_def])
+
+val lookup_fromAList = store_thm ("lookup_fromAList",
+  ``!x v ls. lookup x (fromAList ls) = SOME v ==> MEM (x,v) ls``,
+  strip_tac>>strip_tac>>Induct>>
+  fs[fromAList_def,lookup_def]>>
+  Cases_on`h`>>
+    Cases_on`q=x`>>
+      rw[lookup_def,fromAList_def]>> fs[lookup_insert] >>
+      metis_tac[]
+  )
+
+val MEM_MAP_FST = store_thm ("MEM_MAP_FST",
+``!f v x ls. MEM (f v,x) ls ==> MEM (f v) (MAP FST ls)``,
+     Induct_on `ls` >>
+      fs[]>> 
+      Cases>>
+      rpt strip_tac>>
+      fs[]>>
+      metis_tac[])
+
+val ZIP_CORRECT = store_thm ("ZIP_CORRECT",
+   (*Zipping correctness*)
+``!l v x' f. MEM (v,x') l 
+  ==> MEM (f v,x') (ZIP (MAP (f o FST) l,MAP SND l))``,
+     (Induct_on `l`>>
+     fs[] >>
+     Cases >>
+     rpt strip_tac>>
+     fs[]) )
+
+val ZIP_CORRECT_INJ = store_thm ("ZIP_CORRECT_INJ",
+``!l v x' f. INJ f UNIV UNIV
+  ==> 
+  ((MEM (v,x') l) <=> (MEM (f v,x') (ZIP (MAP (f o FST) l,MAP SND l))))``,
+  Induct_on `l`>>
+  fs[] >>
+  Cases >>
+  rpt strip_tac>>
+  fs[]>>
+  Cases_on `v=q`>-
+    (fs[]>>metis_tac[])>>
+  fs[] >> 
+  `f v <> f q` by
+  fs[INJ_DEF]>>
+  metis_tac[INJ_DEF])
+
+(*Prove that get_var gives the same result under an injective f*)
+val inj_apply_nummap_key = store_thm("inj_apply_nummap_key_invariant",
+  ``!f v s x. INJ f UNIV UNIV /\ get_var v s = x 
+    ==> get_var (f v) (s with locals := apply_nummap_key f s.locals) = x``,
+  rpt strip_tac>>
+  Cases_on `x`>>
+  fs[get_var_def]>-
+   (
+  SPOSE_NOT_THEN ASSUME_TAC>>
+  fs[lookup_NONE_domain] >>
+  IMP_RES_TAC MEM_fromAList>>
+  fs[MAP_ZIP]>>
+  fs[MEM_MAP]>>
+  Cases_on `y`>>
+    fs[MEM_toAList]>>
+    Cases_on `q=v`>- 
+      fs[domain_lookup] 
+    >> fs[INJ_DEF] >>metis_tac[]) >> 
+  (*FIND A NEATER WAY*)
+  Q.ABBREV_TAC `ls = (ZIP
+        (MAP (f o FST) (toAList s.locals),
+         MAP SND (toAList s.locals)))` >>
+  Cases_on `lookup (f v) (fromAList ls)` >> rw[] 
+   >-(
+    fs[lookup_NONE_domain]>>
+    ASSUME_TAC MEM_fromAList>>
+    first_x_assum(qspecl_then [`ls`,`f v`] assume_tac)>>
+    IMP_RES_TAC MEM_toAList>>
+  (*Zipping correctness*)
+  ASSUME_TAC (INST_TYPE [``:'c``|-> ``:num``,``:'b``|->``:'a word_loc``,``:'a``|-> ``:num``] ZIP_CORRECT) >>
+ first_x_assum(qspecl_then [`toAList s.locals`,`v`,`x'`,`f`] mp_tac)>>
+  strip_tac>>
+  (*HOW TO: reapply an abbrev???*)
+  Q.UNABBREV_TAC `ls`>>
+  Q.ABBREV_TAC `ls = (ZIP
+        (MAP (f o FST) (toAList s.locals),
+         MAP SND (toAList s.locals)))` >>
+  ASSUME_TAC (INST_TYPE [``:'a`` |-> ``:num``,``:'b``|->``:num``,
+                         ``:'c``|->``:'a word_loc``] MEM_MAP_FST)>>
+  first_x_assum(qspecl_then [`f`,`v`,`x'`,`ls`] assume_tac)>>
+  metis_tac[])>>
+  ASSUME_TAC (INST_TYPE [``:'a`` |->``:'a word_loc``] lookup_fromAList) >>
+  first_x_assum (qspecl_then [`f v`,`x`,`ls`] assume_tac) >>
+  `MEM (v,x') (toAList s.locals)` by metis_tac[MEM_toAList] >>
+  `MEM (f v,x') ls` by metis_tac[ZIP_CORRECT]>>
+
+  `!y. MEM (v,y) (toAList s.locals) ==> y=x'` by
+    (rw[] >> fs[MEM_toAList]) >>
+  `MEM (f v,x) ls` by metis_tac[] >> 
+   ASSUME_TAC (INST_TYPE [``:'c``|-> ``:num``,``:'b``|->``:'a word_loc``,``:'a``|-> ``:num``] ZIP_CORRECT_INJ)>>
+   first_x_assum (qspecl_then [`toAList s.locals`,`v`] assume_tac) >>
+   first_assum(qspecl_then [`x'`,`f`] assume_tac)>>
+   first_assum(qspecl_then [`x`,`f`] assume_tac)>>
+   metis_tac[]) 
+ 
+
+    metis_tac[MEM_toAList,lookup_def,spt_eq_thm]
+   rw[]>>
+    Q.UNABBREV_TAC `ls`>>
+    ASSUME_TAC ZIP_CORRECT_INJ>>
+
+  metis_tac[ZIP_CORRECT_INJ]
+  rw[]>>
+   
+
+ SPOSE_NOT_THEN ASSUME_TAC>>
+   metis_tac[INJ_DEF]
+
+  
+
+  SPOSE_NOT_THEN ASSUME_TAC>>  
+  ASSUME_TAC (INST_TYPE [``:'a`` |-> ``:'a word_loc``] domain_lookup)>>
+  first_x_assum(qspecl_then [`fromAList ls`,`f v`] assume_tac)>>
+  ASSUME_TAC MEM_fromAList>>
+  `?v'. lookup (f v) (fromAList ls) = SOME v'` by metis_tac[] >>
+  fs[] >>
+  first_x_assum(qspecl_then [`ls`,`f v`] assume_tac)>>
+  `MEM (f v) (MAP FST ls)` by metis_tac[] >>
+  Q.UNABBREV_TAC `ls`>>
+  fs[MAP_ZIP]>>
+  fs[MEM_MAP] >>
+  Cases_on`y` >>
+    Cases_on`q=v`>-
+      
+  
+  metis_tac[MAP_ZIP, MEM_MAP, INJ_DEF,MEM_fromAList]
+
+
+  HINT_EXISTS_TAC
+
+lookup_NONE_domain >>
+  
+  IMP_RES_TAC MEM_fromAList>>
+  fs[MAP_ZIP]>>
+  fs[MEM_MAP]>>
+
+  Cases_on `y`>>
+    fs[MEM_toAList]>>
+    Cases_on `q=v`>- 
+      fs[domain_lookup] 
+    >> fs[INJ_DEF] >>metis_tac[]) >> 
+
+
+  IMP_RES_TAC MEM_MAP_FST>>
+   
+  
+  metis_tac[
+  fs[] >> pop_assum mp_tac>>
+  simp[] >> strip_tac>>
+  `!x t. lookup x t <> NONE <=> x IN domain t` by
+  fs[lookup_NONE_domain,domain_lookup]>>
+  first_x_assum(qspecl_then [`v`,`s.locals`] assume_tac) >>
+   
+   
+
+   
+
+
+(*Helpful:
+   traces();
+
+   Goalstack.print_goal_fvs := 1;
+    show_types:=true;
+    show_types:=false;
+ *)
+
+  IMP_RES_TAC MEM_toAList >>
+    ASSUME_TAC MEM_fromAList>>
+  `!ls. MEM (f v,x') ls ==> MEM (f v) (MAP FST ls)` by
+     rpt strip_tac>>
+     fs[MEM_MAP] >>
+     EXISTS_TAC ``(f v,x')``>> simp[])
+
+     metis_tac[]
+       EXISTS_TAC
+                     metis_tac[]
+    Induct_on `ls`>>
+      fs[]>>
+
+
+   )
+
+
+
+  fs[MAP_ZIP]
+  IMP_RES_TAC MEM_MAP>>
+  fs[]>> 
+  first_assum(qspec_then `b` assume_tac)
+
+   IMP_RES_TAC MEM_fromAList >> 
+
+
+      fs[MAP_ZIP,MEM_toAList,domain_lookup] >>
+     rw[] 
+      >> fs[INJ_DEF] >> metis_tac[])
+    
+
+
+
+     metis_tac[MEM_fromAList,MEM_toAList] 
+    strip_tac>>
+     first_assum(qspec_then `ls` assume_tac)
+     first_x_assum(qspec_then `ls` mp_tac) 
+   (*SOME*)
+   >>
+   
+
+ 
+    `lookup v s.locals = NONE ==> ~(v IN domain s.locals)` by
+      fs[domain_lookup,lookup_def]>> 
+   fs[domain_lookup,lookup_NONE_domain]>>
+    Cases_on `
+    rw[fromAList_def] 
+  CONTR_TAC
+
+_CASES_TAC
+  fs[MEM_toAList]
+
+  rw[get_var_def,toAList_def,fromAList_def]
+
+(*Prove that mapping injective f over a prog + initial state variables gives the same result and a new state which contains mapped vars*)
+val inj_apply_color_invariant = store_thm ("inj_apply_color_invariant",
+  ``!prog s s1 f res. wEval(prog,s) = (res,s1) 
+                  /\ INJ f UNIV UNIV
+                  /\ res <> SOME Error
+    ==> wEval(apply_color f prog, 
+              s with locals := apply_nummap_key f s.locals) = 
+        (res,s1 with locals := apply_nummap_key f s1.locals)``,
+
+  ho_match_mp_tac (wEval_ind |> Q.SPEC`UNCURRY P` |> SIMP_RULE (srw_ss())[] |> Q.GEN`P`) >> rw[] >-
+  (*Skip*)
+  fs[wEval_def] >-
+
+  (*Move*)
+
+  fs[MAP_ZIP,wEval_def,get_vars_def,set_vars_def,list_insert_def]>>
+  rw[]>> simp[] >-
+    Cases_on`ALL_DISTINCT (MAP FST moves)` >>
+    fs[]>>
+    Cases_on `get_vars (MAP SND moves) s` >>
+    fs[]>>
+    `!x f. INJ f UNIV UNIV /\ get_vars (MAP SND moves) s = SOME x ==>
+     get_vars (MAP (f o SND) moves) (s with locals := apply_nummap_key f s.locals) = SOME x` by
+    Induct_on `moves`>>
+      fs[get_vars_def]>>
+    rpt strip_tac >>
+    Cases_on`get_var (SND h) s`>> fs[]>>
+    rw[get_var_def]>> 
+
+    rw[fromAList_def]
+    rw[get_vars_def]>>
+       Induct_on `moves`>-
+         fs[get_vars_def] >>
+       rw[get_vars_def,get_var_def]>>
+
+  Induct_on `moves`>-
+   (>>
+   strip_tac>>
+   rw[word_state_updates_eq_literal])>>
+
+  rw[wEval_def,apply_color_def] >
+   fs[MAP_ZIP,get_vars_def,apply_nummap_key_def]
+
+  
 
 (*Result of adding a move using injective f is invariant
 Resulting state might have extra locals (depending on f) 
@@ -156,6 +436,7 @@ val inj_move_conv_invariant = store_thm ("move_invariant",
          /\ (!x y. lookup x s1.locals = y ==> lookup (f x) s2.locals = y)
          (*Other state conditions TODO *)
          /\ (?l. s2 = s1 with locals := l) ``,
+
   ho_match_mp_tac (wEval_ind |> Q.SPEC`UNCURRY P` |> SIMP_RULE (srw_ss())[] |> Q.GEN`P`) >>
   rw[] >>
   
